checkpoint

pulse/ulib/experimental/Steel.Heap.fsti
@@ -335,13 +335,21 @@ val weaken (p q r:slprop) (h:heap u#a)
 
 (**** Actions *)
 
+(** An abstract predicate classifying a "full" heap, i.e., the entire
+    heap of the executing program, not just a fragment of it *)
+val full_heap_pred : heap -> prop
+
+let full_heap = h:heap { full_heap_pred h }
+
+let full_hheap fp = h:hheap fp { full_heap_pred h }
+
 (**
   This modules exposes a preorder that is respected for every well-formed update of the heap.
   The preorder represents the fact that once a reference is allocated, its type and PCM cannot
   change and the trace of values contained in the PCM respects the preorder induced by the
   PCM (see Steel.Preorder).
 *)
-val heap_evolves : FStar.Preorder.preorder heap
+val heap_evolves : FStar.Preorder.preorder full_heap
 
 (**
   This predicate allows us to maintain an allocation counter, as all references above [a]
@@ -358,7 +366,7 @@ val weaken_free_above (h:heap) (a b:nat)
   the heap specification of the action before and after.
 *)
 let pre_action (fp:slprop u#a) (a:Type u#b) (fp':a -> slprop u#a) =
-  hheap fp -> (x:a & hheap (fp' x))
+  full_hheap fp -> (x:a & full_hheap (fp' x))
 
 (**
   We only want to consider heap updates that are "frame-preserving", meaning that they only
@@ -375,7 +383,7 @@ let is_frame_preserving
   (#fp': a -> slprop u#b)
   (f:pre_action fp a fp')
   =
-  forall (frame: slprop u#b) (h0:hheap (fp `star` frame)).
+  forall (frame: slprop u#b) (h0:full_hheap (fp `star` frame)).
      (affine_star fp frame h0;
       let (| x, h1 |) = f h0 in
       interp (fp' x `star` frame) h1 /\
@@ -387,7 +395,7 @@ let is_frame_preserving
   Two heaps [h0] and [h1] are frame-related if you can get from [h0] to [h1] with a
   frame-preserving update.
 *)
-let frame_related_heaps (h0 h1:heap) (fp0 fp1 frame:slprop) (allocates:bool) =
+let frame_related_heaps (h0 h1:full_heap) (fp0 fp1 frame:slprop) (allocates:bool) =
   interp (fp0 `star` frame) h0 ==>
   interp (fp1 `star` frame) h1 /\
   heap_evolves h0 h1 /\
@@ -407,7 +415,7 @@ let action_framing
   (#fp: slprop u#b)
   (#fp': a -> slprop u#b)
   ($f:action fp a fp')
-  (frame:slprop) (h0:hheap (fp `star` frame))
+  (frame:slprop) (h0:full_hheap (fp `star` frame))
     : Lemma (
       affine_star fp frame h0;
       let (| x, h1 |) = f h0 in
@@ -418,23 +426,24 @@ let action_framing
   emp_unit fp
 
 (** [sel] is a ghost read of the value contained in a heap reference *)
-val sel (#a:Type u#h) (#pcm:pcm a) (r:ref a pcm) (m:hheap (ptr r)) : a
+val sel (#a:Type u#h) (#pcm:pcm a) (r:ref a pcm) (m:full_hheap (ptr r)) : a
 
 (** [sel_v] is a ghost read of the value contained in a heap reference *)
-val sel_v (#a:Type u#h) (#pcm:pcm a) (r:ref a pcm) (v:erased a) (m:hheap (pts_to r v))
+val sel_v (#a:Type u#h) (#pcm:pcm a) (r:ref a pcm) (v:erased a) (m:full_hheap (pts_to r v))
   : v':a{ compatible pcm v v' /\
+          pcm.refine v' /\
           interp (ptr r) m /\
           v' == sel r m }
 
 (** [sel] respect [pts_to] *)
-val sel_lemma (#a:_) (#pcm:_) (r:ref a pcm) (m:hheap (ptr r))
+val sel_lemma (#a:_) (#pcm:_) (r:ref a pcm) (m:full_hheap (ptr r))
   : Lemma (interp (pts_to r (sel r m)) m)
 
 let witnessed_ref (#a:Type u#a)
                   (#pcm:pcm a)
                   (r:ref a pcm)
                   (fact:a -> prop)
-                  (h:heap)
+                  (h:full_heap)
   = interp (ptr r) h /\
     fact (sel r h)
 
@@ -463,7 +472,7 @@ val upd_action
   (#pcm:pcm a)
   (r:ref a pcm)
   (v0:FStar.Ghost.erased a)
-  (v1:a {FStar.PCM.frame_preserving pcm v0 v1})
+  (v1:a {FStar.PCM.frame_preserving pcm v0 v1 /\ pcm.refine v1})
   : action (pts_to r v0) unit (fun _ -> pts_to r v1)
 
 (** Deallocating a reference, by actually replacing its value by the unit of the PCM *)
@@ -471,7 +480,7 @@ val free_action
   (#a:Type u#a)
   (#pcm:pcm a)
   (r:ref a pcm)
-  (v0:FStar.Ghost.erased a {exclusive pcm v0})
+  (v0:FStar.Ghost.erased a {exclusive pcm v0 /\ pcm.refine pcm.p.one})
   : action (pts_to r v0) unit (fun _ -> emp)
 
 
@@ -499,10 +508,10 @@ val extend
   (#pcm:pcm a)
   (x:a{compatible pcm x x})
   (addr:nat)
-  (h:heap{h `free_above_addr` addr})
+  (h:full_heap{h `free_above_addr` addr})
   : (
     r:ref a pcm
-    & h':heap{
+    & h':full_heap{
       (forall (frame: slprop u#a).
         frame_related_heaps h h' emp (pts_to r x) frame (true)) /\
         h' `free_above_addr` (addr + 1) /\
